Prove on RTL's step lemma for memory injection.

sepcomp/backend/RTL_sepcomp.v
@@ -2,7 +2,9 @@ Require Import Coqlib.
 Require Import Maps.
 Require Import Integers.
 Require Import Values.
+Require Import AST.
 Require Import Memory.
+Require Import Globalenvs.
 Require Import Events.
 Require Import Op.
 Require Import Registers.
@@ -11,28 +13,56 @@ Require Import sflib.
 
 Set Implicit Arguments.
 
+Lemma shift_stack_addressing_Int_zero addr:
+  shift_stack_addressing Int.zero addr = addr.
+Proof.
+  destruct addr; auto. simpl.
+  f_equal. apply Int.add_zero_l.
+Qed.
+
+Lemma shift_stack_operation_Int_zero op:
+  shift_stack_operation Int.zero op = op.
+Proof.
+  destruct op; auto. simpl. f_equal.
+  apply shift_stack_addressing_Int_zero.
+Qed.
+
 Lemma inject_separated_refl F m tm:
   inject_separated F F m tm.
 Proof. ii. congruence. Qed.
 
-Lemma val_inject_set_reg:
+Definition regset_inject F rs trs :=
+  forall r, val_inject F rs # r trs # r.
+
+Definition regset_inject_incr F1 F2 rs trs
+           (INCR: inject_incr F1 F2)
+           (INJ: regset_inject F1 rs trs):
+  regset_inject F2 rs trs.
+Proof. ii. eapply val_inject_incr; eauto. Qed.
+
+Lemma regset_inject_val_list_inject F rs trs l
+      (INJ: regset_inject F rs trs):
+  val_list_inject F rs ## l trs ## l.
+Proof. induction l; constructor; auto. Qed.
+
+Lemma regset_inject_set_reg:
   forall F rs rs' r v v',
-  (forall r', val_inject F rs # r' rs' # r') ->
+  regset_inject F rs rs' ->
   val_inject F v v' ->
-  forall r', val_inject F (rs#r <- v) # r' (rs'#r <- v') # r'.
+  regset_inject F (rs#r <- v) (rs'#r <- v').
 Proof.
-  intros. rewrite ? Regmap.gsspec. destruct (peq r' r); auto.
+  ii. rewrite ? Regmap.gsspec. destruct (peq r0 r); auto.
 Qed.
 
-Lemma val_inject_init_regs F args args' params
+Lemma regset_inject_init_regs F args args' params
       (ARGS: val_list_inject F args args'):
-  forall r, val_inject F (init_regs args params) # r (init_regs args' params) # r.
+  regset_inject F (init_regs args params) (init_regs args' params).
 Proof.
-  revert args args' ARGS. induction params; simpl; intros.
+  revert args args' ARGS. induction params; simpl; ii.
   - rewrite ? Regmap.gi. auto.
   - inv ARGS.
     + rewrite ? Regmap.gi. auto.
-    + apply val_inject_set_reg; auto.
+    + apply regset_inject_set_reg; auto.
 Qed.
 
 Definition is_normal (s:state): bool :=
@@ -67,18 +97,20 @@ Lemma is_normal_steps
       ge s f sp pc1 rs1 m1 pc2 rs2 m2 tr
       tge ts tsp trs1 tm1
       F1
+      (SYMBOL: forall (s: ident), Genv.find_symbol tge s = Genv.find_symbol ge s)
+      (VARINFO: forall b, Genv.find_var_info tge b = Genv.find_var_info ge b)
       (NORMAL1: is_normal (State s f (Vptr sp Int.zero) pc1 rs1 m1))
       (STEP: step ge (State s f (Vptr sp Int.zero) pc1 rs1 m1) tr (State s f (Vptr sp Int.zero) pc2 rs2 m2))
       (SP: F1 sp = Some(tsp, 0))
       (PRES1: meminj_preserves_globals ge F1)
-      (REGSET1: forall r, val_inject F1 rs1#r trs1#r)
+      (REGSET1: regset_inject F1 rs1 trs1)
       (MEM1: Mem.inject F1 m1 tm1):
   exists F2 trs2 tm2,
     <<TSTEP: step tge (State ts f (Vptr tsp Int.zero) pc1 trs1 tm1) tr (State ts f (Vptr tsp Int.zero) pc2 trs2 tm2)>> /\
     <<MAXPERM: forall b ofs p, Mem.valid_block m1 b -> Mem.perm m2 b ofs Max p -> Mem.perm m1 b ofs Max p>> /\
     <<MAXPERM': forall b ofs p, Mem.valid_block tm1 b -> Mem.perm tm2 b ofs Max p -> Mem.perm tm1 b ofs Max p>> /\
     <<UNCHANGED: Mem.unchanged_on (loc_out_of_reach F1 m1) tm1 tm2>> /\
-    <<REGSET2: forall r, val_inject F2 rs2#r trs2#r>> /\
+    <<REGSET2: regset_inject F2 rs2 trs2>> /\
     <<MEM2: Mem.inject F2 m2 tm2>> /\
     <<INCR: inject_incr F1 F2>> /\
     <<SEP: inject_separated F1 F2 m1 tm1>>.
@@ -89,40 +121,56 @@ Proof.
     + apply Mem.unchanged_on_refl.
     + apply inject_separated_refl.
   - exploit eval_operation_inject; try apply H10; eauto.
-    { instantiate (1 := trs1 ## l). admit. }
-    intro. des.
+    { apply regset_inject_val_list_inject. eauto. }
+    rewrite shift_stack_operation_Int_zero. intro. des.
     eexists. eexists. eexists. splits; eauto.
     + eapply exec_Iop; eauto.
-      instantiate (1 := v2). admit.
+      erewrite eval_operation_preserved; eauto.
     + apply Mem.unchanged_on_refl.
-    + apply val_inject_set_reg; auto.
+    + apply regset_inject_set_reg; auto.
     + apply inject_separated_refl.
   - exploit eval_addressing_inject; try apply H10; eauto.
-    { instantiate (1 := trs1 ## l). admit. }
-    intro. des.
+    { apply regset_inject_val_list_inject. eauto. }
+    rewrite shift_stack_addressing_Int_zero. intro. des.
     exploit Mem.loadv_inject; eauto.
     intro. des.
     eexists. eexists. eexists. splits; eauto.
     + eapply exec_Iload; eauto.
-      admit.
+      erewrite eval_addressing_preserved; eauto.
     + apply Mem.unchanged_on_refl.
-    + apply val_inject_set_reg; auto.
+    + apply regset_inject_set_reg; auto.
     + apply inject_separated_refl.
   - exploit eval_addressing_inject; try apply H10; eauto.
-    { instantiate (1 := trs1 ## l). admit. }
-    intro. des.
+    { apply regset_inject_val_list_inject. eauto. }
+    rewrite shift_stack_addressing_Int_zero. intro. des.
     exploit Mem.storev_mapped_inject; eauto.
     intro. des.
     eexists. eexists. exists n2. splits; eauto.
     + eapply exec_Istore; eauto.
-      admit.
-    + admit. (* perm? *)
-    + admit. (* perm? *)
-    + admit. (* unchanged_on loc_out_of_reach *)
+      erewrite eval_addressing_preserved; eauto.
+    + destruct a0; inv H11. intros. eapply Mem.perm_store_2; eauto.
+    + destruct v2; inv H1. intros. eapply Mem.perm_store_2; eauto.
+    + destruct v2; inv H1. eapply Mem.store_unchanged_on; eauto. ii.
+      inv H0; [|inv H11]. simpl in *.
+      exploit Mem.store_valid_access_3; try apply H11; eauto. intros VA1.
+      exploit Mem.store_valid_access_1; try apply H11; eauto. intros VA2.
+      destruct VA1 as [PERM1 _], VA2 as [PERM2 _].
+      erewrite Mem.address_inject in H1; eauto.
+      * eapply H3; eauto.
+        apply Mem.perm_cur_max. eapply Mem.perm_implies; [|apply perm_any_N]. apply PERM1. xomega.
+      * apply PERM2. xomega.
     + apply inject_separated_refl.
-  - admit. (* external call *)
+  - exploit external_call_mem_inject; eauto.
+    { apply regset_inject_val_list_inject. eauto. }
+    intro. des. eexists. eexists. eexists. splits; try apply H1; eauto.
+    + econs; eauto.
+      eapply external_call_symbols_preserved; eauto. 
+    + intros. eapply external_call_max_perm; eauto.
+    + intros. eapply external_call_max_perm; eauto.
+    + apply regset_inject_set_reg; auto.
+      eapply regset_inject_incr; eauto.
   - exploit eval_condition_inject; try apply H10; eauto.
-    { instantiate (1 := trs1 ## l). admit. }
+    { apply regset_inject_val_list_inject. eauto. }
     intro.
     eexists. eexists. eexists. splits; eauto.
     + eapply exec_Icond; eauto.
